examples/seq-hoh/ImplSpec.s.dfy
@@ -1,0 +1,66 @@
+include "StateMachine.s.dfy"
+
+abstract module DonateImplSpec {
+  import opened SM : StateMachine
+  import opened Options
+
+  method donate(victim: nat, linear ticket: StateObject)
+  returns (outidx: Option<nat>, linear stub: StateObject)
+  requires exists tid :: ticket == donate_ticket(tid, victim)
+  ensures exists tid :: stub == donate_stub(tid, outidx)
+
+  // An infinite number of transform functions
+
+  method {:axiom} transform_2_1(
+      linear a1: StateObject,
+      linear a2: StateObject,
+      ghost b: StateObject)
+  returns (linear b': StateObject)
+  requires transform(multiset{a1, a2}, multiset{b})
+  ensures b' == b
+
+  method {:axiom} transform_3_3(
+      linear a1: StateObject,
+      linear a2: StateObject,
+      linear a3: StateObject,
+      ghost b1: StateObject,
+      ghost b2: StateObject,
+      ghost b3: StateObject)
+  returns (
+    linear b1': StateObject,
+    linear b2': StateObject,
+    linear b3': StateObject)
+  requires transform(multiset{a1, a2, a3}, multiset{b1, b2, b3})
+  ensures b1' == b1
+  ensures b2' == b2
+  ensures b3' == b3
+
+  method {:axiom} transform_3_2(
+      linear a1: StateObject,
+      linear a2: StateObject,
+      linear a3: StateObject,
+      ghost b1: StateObject,
+      ghost b2: StateObject)
+  returns (
+    linear b1': StateObject,
+    linear b2': StateObject)
+  requires transform(multiset{a1, a2, a3}, multiset{b1, b2})
+  ensures b1' == b1
+  ensures b2' == b2
+
+  method {:axiom} transform_2_3(
+      linear a1: StateObject,
+      linear a2: StateObject,
+      ghost b1: StateObject,
+      ghost b2: StateObject,
+      ghost b3: StateObject)
+  returns (
+    linear b1': StateObject,
+    linear b2': StateObject,
+    linear b3': StateObject)
+  requires transform(multiset{a1, a2}, multiset{b1, b2, b3})
+  ensures b1' == b1
+  ensures b2' == b2
+  ensures b3' == b3
+
+}
